Superposition_Calculus/FSet_Extra.thy
@@ -1,0 +1,21 @@
+theory FSet_Extra
+  imports "HOL-Library.FSet"
+begin
+
+locale finite_set =
+  fixes set :: "'b \<Rightarrow> 'a set"
+  assumes finite_set [simp]: "\<And>b. finite (set b)"
+begin
+
+abbreviation finite_set :: "'b \<Rightarrow> 'a fset" where 
+  "finite_set b \<equiv> Abs_fset (set b)"
+
+lemma finite_set': "set b \<in> {A. finite A}"
+  by simp
+
+lemma fset_finite_set [simp]: "fset (finite_set b) = set b"
+  using Abs_fset_inverse[OF finite_set'].
+
+end
+
+end
