Superposition_Calculus/Functional_Substitution.thy
@@ -1,0 +1,232 @@
+theory Functional_Substitution
+  imports
+    Abstract_Substitution.Substitution
+    FSet_Extra
+begin
+
+locale all_subst_ident_iff_ground =
+  fixes is_ground :: "'expr \<Rightarrow> bool" and subst :: "'expr \<Rightarrow> 'subst \<Rightarrow> 'expr"
+  assumes
+    all_subst_ident_iff_ground: "\<And>expr. is_ground expr \<longleftrightarrow> (\<forall>\<sigma>. subst expr \<sigma> = expr)" and
+    exists_non_ident_subst:
+      "\<And>expr S. finite S \<Longrightarrow> \<not>is_ground expr \<Longrightarrow> \<exists>\<sigma>. subst expr \<sigma> \<noteq> expr \<and> subst expr \<sigma> \<notin> S"
+
+locale finite_variables = finite_set vars 
+  for vars :: "'expr \<Rightarrow> 'var set"
+begin
+
+lemmas finite_vars = finite_set finite_set'
+lemmas fset_finite_vars = fset_finite_set
+
+abbreviation "finite_vars \<equiv> finite_set"
+
+end
+
+locale functional_substitution = substitution _ _ subst "\<lambda>a. vars a = {}" 
+  for
+    subst :: "'expr \<Rightarrow> ('var \<Rightarrow> 'base) \<Rightarrow> 'expr" (infixl "\<cdot>" 70) and
+    vars :: "'expr \<Rightarrow> 'var set" +
+  assumes 
+    subst_eq: "\<And>expr \<sigma> \<tau>. (\<And>x. x \<in> (vars expr) \<Longrightarrow> \<sigma> x = \<tau> x) \<Longrightarrow> expr \<cdot> \<sigma> = expr \<cdot> \<tau>"
+begin
+
+abbreviation is_ground where "is_ground expr \<equiv> vars expr = {}"
+
+definition vars_set :: "'expr set \<Rightarrow> 'var set" where
+  "vars_set exprs \<equiv> \<Union>expr \<in> exprs. vars expr"
+
+lemma subst_reduntant_upd [simp]:
+  assumes "var \<notin> vars expr"
+  shows "expr \<cdot> \<sigma>(var := update) = expr \<cdot> \<sigma>"
+  using assms subst_eq
+  by fastforce
+
+lemma subst_reduntant_if [simp]: 
+  assumes "vars expr \<subseteq> vars'"
+  shows "expr \<cdot> (\<lambda>var. if var \<in> vars' then \<sigma> var else \<sigma>' var) = expr \<cdot> \<sigma>"
+  using assms 
+  by (smt (verit, best) subset_eq subst_eq)
+
+lemma subst_reduntant_if' [simp]: 
+  assumes "vars expr \<inter> vars' = {}"  
+  shows "expr \<cdot> (\<lambda>var. if var \<in> vars' then \<sigma>' var else \<sigma> var) = expr \<cdot> \<sigma>"
+  using assms subst_eq 
+  unfolding disjoint_iff
+  by presburger
+
+lemma subst_cannot_unground:
+  assumes "\<not>is_ground (expr \<cdot> \<sigma>)"  
+  shows "\<not>is_ground expr"
+  using assms by force
+
+end
+
+locale grounding = functional_substitution where vars = vars and id_subst = id_subst
+  for vars :: "'expr \<Rightarrow> 'var set" and id_subst :: "'var \<Rightarrow> 'base" +
+  fixes to_ground :: "'expr \<Rightarrow> 'expr\<^sub>G" and from_ground :: "'expr\<^sub>G \<Rightarrow> 'expr"
+  assumes 
+    range_from_ground_iff_is_ground: "{expr. is_ground expr} = range from_ground" and
+    from_ground_inverse [simp]: "\<And>expr\<^sub>G. to_ground (from_ground expr\<^sub>G) = expr\<^sub>G"
+begin
+
+definition groundings ::"'expr \<Rightarrow> 'expr\<^sub>G set" where
+  "groundings expr = { to_ground (expr \<cdot> \<gamma>) | \<gamma>. is_ground (expr \<cdot> \<gamma>) }"
+
+lemma to_ground_from_ground_id: "to_ground \<circ> from_ground = id"
+  using from_ground_inverse
+  by auto
+
+lemma surj_to_ground: "surj to_ground"
+  using from_ground_inverse
+  by (metis surj_def)
+
+lemma inj_from_ground: "inj_on from_ground domain\<^sub>G"
+  by (metis from_ground_inverse inj_on_inverseI)
+ 
+lemma inj_on_to_ground: "inj_on to_ground (from_ground ` domain\<^sub>G)"
+  unfolding inj_on_def
+  by simp
+
+lemma bij_betw_to_ground: "bij_betw to_ground (from_ground ` domain\<^sub>G) domain\<^sub>G"
+  by (smt (verit, best) bij_betwI' from_ground_inverse image_iff)
+
+lemma bij_betw_from_ground: "bij_betw from_ground domain\<^sub>G (from_ground ` domain\<^sub>G)"
+  by (simp add: bij_betw_def inj_from_ground)
+
+lemma ground_is_ground [simp, intro]: "is_ground (from_ground expr\<^sub>G)"
+  using range_from_ground_iff_is_ground
+  by blast
+
+lemma is_ground_iff_range_from_ground: "is_ground expr \<longleftrightarrow> expr \<in> range from_ground"
+  using range_from_ground_iff_is_ground
+  by auto
+
+lemma to_ground_inverse [simp]: 
+  assumes "is_ground expr"
+  shows "from_ground (to_ground expr) = expr"
+  using inj_on_to_ground from_ground_inverse is_ground_iff_range_from_ground assms
+  unfolding inj_on_def
+  by blast
+
+corollary obtain_grounding: 
+  assumes "is_ground expr"
+  obtains expr\<^sub>G where "from_ground expr\<^sub>G = expr"
+  using to_ground_inverse assms 
+  by blast
+
+end
+
+locale base_functional_substitution = functional_substitution 
+  where id_subst = id_subst and vars = vars
+  for id_subst :: "'var \<Rightarrow> 'expr" and vars :: "'expr \<Rightarrow> 'var set" +
+  assumes
+    is_grounding_iff_vars_grounded:
+      "\<And>expr. is_ground (expr \<cdot> \<gamma>) \<longleftrightarrow> (\<forall>var \<in> vars expr. is_ground (\<gamma> var))" and
+    ground_exists: "\<exists>expr. is_ground expr"
+begin 
+
+lemma obtain_ground_subst:
+  obtains \<gamma>
+  where "is_ground_subst \<gamma>"
+proof-
+  obtain expr\<^sub>G where "is_ground expr\<^sub>G"
+    using ground_exists by blast
+
+  then have "is_ground_subst  (\<lambda>_. expr\<^sub>G)"
+    by (simp add: is_grounding_iff_vars_grounded is_ground_subst_def)
+
+  then show ?thesis
+    using that
+    by simp
+qed
+
+lemma ground_subst_extension:
+  assumes "is_ground (expr \<cdot> \<gamma>)"
+  obtains \<gamma>'
+  where "expr \<cdot> \<gamma> = expr \<cdot> \<gamma>'" and "is_ground_subst \<gamma>'"
+proof-
+  obtain \<gamma>'' where 
+    \<gamma>'': "is_ground_subst \<gamma>''"
+    using obtain_ground_subst
+    by blast
+                    
+  define \<gamma>' where 
+    \<gamma>':  "\<gamma>' = (\<lambda>var. if var \<in> vars expr then \<gamma> var else \<gamma>'' var)"
+
+  have "is_ground_subst \<gamma>'"
+    using assms \<gamma>'' is_grounding_iff_vars_grounded
+    unfolding \<gamma>' is_ground_subst_def
+    by simp
+
+  moreover have "expr \<cdot> \<gamma> = expr \<cdot> \<gamma>'"
+    unfolding \<gamma>'
+    using subst_eq by presburger
+
+  ultimately show ?thesis
+    using that
+    by blast
+qed
+
+lemma ground_subst_upd [simp]:
+  assumes "is_ground update" "is_ground (expr \<cdot> \<gamma>)" 
+  shows "is_ground (expr \<cdot> \<gamma>(var := update))"
+  using assms is_grounding_iff_vars_grounded by auto
+
+lemma variable_grounding:
+  assumes "is_ground (expr \<cdot> \<gamma>)" "var \<in> vars expr" 
+  shows "is_ground (\<gamma> var)"
+  using assms is_grounding_iff_vars_grounded 
+  by blast
+
+end
+
+locale based_functional_substitution = 
+  base: base_functional_substitution where subst = base_subst and vars = base_vars + 
+  functional_substitution where vars = vars 
+for 
+  base_subst :: "'base \<Rightarrow> ('var \<Rightarrow> 'base) \<Rightarrow> 'base" and 
+  base_vars and 
+  vars :: "'expr \<Rightarrow> 'var set" +
+assumes
+  ground_subst_iff_base_ground_subst [simp]: "is_ground_subst \<gamma> \<longleftrightarrow> base.is_ground_subst \<gamma>" and
+  is_grounding_iff_vars_grounded: 
+    "\<And>expr. is_ground (expr \<cdot> \<gamma>) \<longleftrightarrow> (\<forall>var \<in> vars expr. base.is_ground (\<gamma> var))"
+begin
+
+lemma obtain_ground_subst:
+  obtains \<gamma> 
+  where "is_ground_subst \<gamma>"
+  using base.obtain_ground_subst by auto
+
+lemma ground_subst_extension:
+  assumes "is_ground (expr \<cdot> \<gamma>)"
+  obtains \<gamma>'
+  where "expr \<cdot> \<gamma> = expr \<cdot> \<gamma>'" and "is_ground_subst \<gamma>'"
+  using obtain_ground_subst assms
+  by (metis all_subst_ident_if_ground is_ground_subst_comp_right subst_comp_subst)
+
+lemma ground_subst_extension':
+  assumes "is_ground (expr \<cdot> \<gamma>)"
+  obtains \<gamma>'
+  where "expr \<cdot> \<gamma> = expr \<cdot> \<gamma>'" and "base.is_ground_subst \<gamma>'"
+  using ground_subst_extension assms
+  by auto
+
+lemma ground_subst_upd [simp]:
+  assumes "base.is_ground update" "is_ground (expr \<cdot> \<gamma>)" 
+  shows "is_ground (expr \<cdot> \<gamma>(var := update))"
+  using base.ground_subst_upd assms is_grounding_iff_vars_grounded by simp  
+
+lemma ground_exists: "\<exists>expr. is_ground expr"
+  using base.ground_exists
+  by (meson is_grounding_iff_vars_grounded)
+
+lemma variable_grounding:
+  assumes "is_ground (expr \<cdot> \<gamma>)" "var \<in> vars expr" 
+  shows "base.is_ground (\<gamma> var)"
+  using assms is_grounding_iff_vars_grounded 
+  by blast
+
+end
+
+end
