Superposition_Calculus/Functional_Substitution_Lifting.thy
@@ -1,0 +1,392 @@
+theory Functional_Substitution_Lifting
+  imports Functional_Substitution
+begin
+
+locale functional_substitution_lifting = 
+  sub: functional_substitution
+  where subst = sub_subst and vars = sub_vars
+  for
+    sub_vars :: "'sub \<Rightarrow> 'var set" and
+    sub_subst :: "'sub \<Rightarrow> ('var \<Rightarrow> 'base) \<Rightarrow> 'sub" +
+  fixes
+    map :: "('sub \<Rightarrow> 'sub) \<Rightarrow> 'expr \<Rightarrow> 'expr" and
+    to_set :: "'expr \<Rightarrow> 'sub set"
+  assumes
+    map_comp: "\<And>expr f g. map (f \<circ> g) expr = map f (map g expr)" and
+    map_id: "map id expr = expr" and
+    map_cong: 
+      "\<And>expr f g. (\<And>sub. sub \<in> to_set expr \<Longrightarrow> f sub = g sub) \<Longrightarrow> map f expr = map g expr" and
+    to_set_map: "\<And>expr f. to_set (map f expr) = f ` to_set expr" and
+    exists_expression: "\<And>sub. \<exists>expr. sub \<in> to_set expr" 
+begin
+
+definition vars :: "'expr \<Rightarrow> 'var set" where
+  "vars expr \<equiv> \<Union> (sub_vars ` to_set expr)"
+
+notation sub_subst (infixl "\<cdot>\<^sub>s" 70)
+
+definition subst :: "'expr \<Rightarrow> ('var \<Rightarrow> 'base) \<Rightarrow> 'expr" (infixl "\<cdot>" 70) where
+  "expr \<cdot> \<sigma> \<equiv> map (\<lambda>sub. sub \<cdot>\<^sub>s \<sigma>) expr"
+
+lemma map_id_cong: 
+  assumes "\<And>sub. sub \<in> to_set expr \<Longrightarrow> f sub = sub"  
+  shows "map f expr = expr"
+  using map_cong map_id assms
+  unfolding id_def
+  by metis
+
+lemma to_set_map_not_ident: 
+  assumes "sub \<in> to_set expr" "f sub \<notin> to_set expr" 
+  shows "map f expr \<noteq> expr"
+  using assms
+  by (metis rev_image_eqI to_set_map)
+
+lemma subst_in_to_set_subst:
+  assumes "sub \<in> to_set expr" 
+  shows "sub \<cdot>\<^sub>s \<sigma> \<in> to_set (expr \<cdot> \<sigma>)"
+  unfolding subst_def to_set_map
+  using assms
+  by simp
+
+sublocale functional_substitution where subst = "(\<cdot>)" and vars = vars
+proof unfold_locales
+  fix expr \<sigma>\<^sub>1 \<sigma>\<^sub>2
+
+  show "expr \<cdot> (\<sigma>\<^sub>1 \<odot> \<sigma>\<^sub>2) = expr \<cdot> \<sigma>\<^sub>1 \<cdot> \<sigma>\<^sub>2"
+    unfolding subst_def map_comp[symmetric] comp_apply sub.subst_comp_subst
+    ..
+next
+  fix expr
+  show "expr \<cdot> id_subst = expr"
+    using map_id
+    unfolding subst_def sub.subst_id_subst id_def.
+next
+  fix expr
+  assume "vars expr = {}"
+  then show "\<forall>\<sigma>. expr \<cdot> \<sigma> = expr"
+    unfolding vars_def subst_def    
+    using map_id_cong
+    by simp
+next
+  fix expr and \<sigma>\<^sub>1 \<sigma>\<^sub>2 :: "'var \<Rightarrow> 'base"
+  assume "\<And>var. var \<in> vars expr \<Longrightarrow> \<sigma>\<^sub>1 var = \<sigma>\<^sub>2 var"
+
+  then show "expr \<cdot> \<sigma>\<^sub>1 = expr \<cdot> \<sigma>\<^sub>2"
+    unfolding vars_def subst_def
+    using map_cong sub.subst_eq
+    by (meson UN_I)
+qed
+
+lemma ground_subst_iff_sub_ground_subst [simp]: "is_ground_subst \<gamma> \<longleftrightarrow> sub.is_ground_subst \<gamma>"
+proof(unfold is_ground_subst_def sub.is_ground_subst_def, intro iffI allI)
+  fix sub 
+  assume all_ground: "\<forall>expr. is_ground (expr \<cdot> \<gamma>)"
+  show "sub.is_ground (sub \<cdot>\<^sub>s \<gamma>)"
+  proof(rule ccontr)
+    assume sub_not_ground: "\<not>sub.is_ground (sub \<cdot>\<^sub>s \<gamma>)"
+
+    then obtain expr where "sub \<in> to_set expr"
+      using exists_expression by auto
+
+    then have "\<not>is_ground (expr \<cdot> \<gamma>)"
+      using sub_not_ground to_set_map 
+      unfolding subst_def vars_def
+      by auto
+
+    then show False
+      using all_ground
+      by blast
+  qed
+next
+  fix expr
+  assume "\<forall>sub. sub.is_ground (sub \<cdot>\<^sub>s \<gamma>)"
+
+  then show "is_ground (expr \<cdot> \<gamma>)"
+    unfolding vars_def subst_def
+    using to_set_map
+    by simp
+qed
+
+lemma to_set_is_ground [intro]:
+  assumes "sub \<in> to_set expr" "is_ground expr"
+  shows "sub.is_ground sub"
+  using assms
+  by (simp add: vars_def)
+
+lemma to_set_is_ground_subst:
+  assumes "sub \<in> to_set expr"  "is_ground (expr \<cdot> \<gamma>)"  
+  shows "sub.is_ground (sub \<cdot>\<^sub>s \<gamma>)"
+  using assms
+  by (meson subst_in_to_set_subst to_set_is_ground)
+
+lemma subst_empty:
+  assumes "to_set expr' = {}"
+  shows "expr \<cdot> \<sigma> = expr' \<longleftrightarrow> expr = expr'"
+  using assms map_id_cong subst_def to_set_map 
+  by fastforce
+
+lemma empty_is_ground:
+  assumes "to_set expr = {}"  
+  shows "is_ground expr"
+  using assms
+  by (simp add: vars_def)
+
+end
+
+locale based_functional_substitution_lifting = 
+  base: base_functional_substitution 
+  where subst = base_subst and vars = base_vars +
+  functional_substitution_lifting
+  where to_set = to_set
+  for base_subst :: "'base \<Rightarrow> ('var \<Rightarrow> 'base) \<Rightarrow> 'base" and base_vars 
+    and to_set :: "'expr \<Rightarrow> 'sub set" +
+  assumes 
+    sub_is_grounding_iff_vars_grounded: 
+      "\<And>expr \<gamma>. sub.is_ground (expr \<cdot>\<^sub>s \<gamma>) \<longleftrightarrow> (\<forall>var \<in> sub_vars expr. base.is_ground (\<gamma> var))" and
+    sub_ground_subst_iff_base_ground_subst: "\<And>\<gamma>. sub.is_ground_subst \<gamma> \<longleftrightarrow> base.is_ground_subst \<gamma>"
+begin
+
+lemma is_grounding_iff_vars_grounded: 
+  "is_ground (subst expr \<gamma>) \<longleftrightarrow> (\<forall>var \<in> vars expr. base.is_ground (\<gamma> var))"
+  using sub_is_grounding_iff_vars_grounded subst_def to_set_map vars_def
+  by auto
+
+lemma ground_subst_iff_base_ground_subst [simp]: 
+  "\<And>\<gamma>. is_ground_subst \<gamma> \<longleftrightarrow> base.is_ground_subst \<gamma>"
+  using sub_ground_subst_iff_base_ground_subst ground_subst_iff_sub_ground_subst by blast
+
+lemma obtain_ground_subst:
+  obtains \<gamma> 
+  where "is_ground_subst \<gamma>"
+  using base.obtain_ground_subst
+  by (meson base.ground_exists is_grounding_iff_vars_grounded is_ground_subst_def that)
+
+lemma ground_subst_extension:
+  assumes "is_ground (expr \<cdot> \<gamma>)"
+  obtains \<gamma>'
+  where "expr \<cdot> \<gamma> = expr \<cdot> \<gamma>'" and "is_ground_subst \<gamma>'"
+  by (metis all_subst_ident_if_ground assms comp_subst.left.monoid_action_compatibility 
+        is_ground_subst_comp_right obtain_ground_subst)
+
+lemma ground_subst_extension':
+  assumes "is_ground (expr \<cdot> \<gamma>)"
+  obtains \<gamma>'
+  where "expr \<cdot> \<gamma> = expr \<cdot> \<gamma>'" and "base.is_ground_subst \<gamma>'"
+  using ground_subst_extension[OF assms]
+  unfolding ground_subst_iff_base_ground_subst.
+ 
+lemma ground_subst_upd [simp]:
+  assumes "base.is_ground update" "is_ground (expr \<cdot> \<gamma>)" 
+  shows "is_ground (expr \<cdot> \<gamma>(var := update))"
+  using assms
+  unfolding is_grounding_iff_vars_grounded
+  by simp
+
+lemma ground_exists: "\<exists>expr. is_ground expr"
+  using base.ground_exists
+  by (meson is_grounding_iff_vars_grounded)
+
+lemma variable_grounding:
+  assumes "is_ground (expr \<cdot> \<gamma>)" "var \<in> vars expr" 
+  shows "base.is_ground (\<gamma> var)"
+  using assms is_grounding_iff_vars_grounded 
+  by blast
+
+end
+
+locale finite_variables_lifting = 
+  sub: finite_variables where vars = "sub_vars :: 'sub \<Rightarrow> 'var set"  +
+  to_set: finite_set where set = "to_set :: 'expr \<Rightarrow> 'sub set" +
+  functional_substitution_lifting
+begin
+
+abbreviation to_fset :: "'expr \<Rightarrow> 'sub fset" where 
+  "to_fset \<equiv> to_set.finite_set"
+
+lemmas finite_to_set = to_set.finite_set to_set.finite_set'
+lemmas fset_to_fset = to_set.fset_finite_set
+
+sublocale finite_variables where vars = vars
+  by unfold_locales (simp add: vars_def)
+
+lemma to_fset_map: "\<And>expr f. to_fset (map f expr) = f |`| to_fset expr"
+  using to_set_map
+  by (metis fset.set_map fset_inverse fset_to_fset)
+
+lemma to_fset_is_ground_subst:
+  assumes "sub |\<in>| to_fset expr"  "is_ground (subst expr \<gamma>)"  
+  shows "sub.is_ground (sub \<cdot>\<^sub>s \<gamma>)"
+  using assms
+  by (simp add: to_set_is_ground_subst)
+
+end
+
+locale grounding_lifting = 
+  functional_substitution_lifting 
+  where sub_vars = sub_vars and sub_subst = sub_subst and map = map + 
+  sub: grounding
+  where vars = sub_vars and subst = sub_subst and to_ground = sub_to_ground and 
+    from_ground = sub_from_ground 
+  for
+    sub_to_ground :: "'sub \<Rightarrow> 'sub\<^sub>G" and 
+    sub_from_ground :: "'sub\<^sub>G \<Rightarrow> 'sub" and
+    sub_vars :: "'sub \<Rightarrow> 'var set" and 
+    sub_subst :: "'sub \<Rightarrow> ('var \<Rightarrow> 'base) \<Rightarrow> 'sub" and
+    map :: "('sub \<Rightarrow> 'sub) \<Rightarrow> 'expr \<Rightarrow> 'expr" +
+  fixes
+    to_ground_map :: "('sub \<Rightarrow> 'sub\<^sub>G) \<Rightarrow> 'expr \<Rightarrow> 'expr\<^sub>G" and
+    from_ground_map :: "('sub\<^sub>G \<Rightarrow> 'sub) \<Rightarrow> 'expr\<^sub>G \<Rightarrow> 'expr" and
+    ground_map :: "('sub\<^sub>G \<Rightarrow> 'sub\<^sub>G) \<Rightarrow> 'expr\<^sub>G \<Rightarrow> 'expr\<^sub>G" and
+    to_set_ground :: "'expr\<^sub>G \<Rightarrow> 'sub\<^sub>G set"
+  assumes 
+    to_set_from_ground_map: 
+      "\<And>expr\<^sub>G f. to_set (from_ground_map f expr\<^sub>G) = f ` to_set_ground expr\<^sub>G" and
+    map_ground_comp: "\<And>expr f g. map (f \<circ> g) expr = from_ground_map f (to_ground_map g expr)" and
+    ground_map_comp: 
+      "\<And>expr\<^sub>G f g. ground_map (f \<circ> g) expr\<^sub>G = to_ground_map f (from_ground_map g expr\<^sub>G)" and
+    ground_map_id: "\<And>expr\<^sub>G. ground_map id expr\<^sub>G = expr\<^sub>G"
+begin
+
+definition to_ground :: "'expr \<Rightarrow> 'expr\<^sub>G" where 
+  "to_ground expr \<equiv> to_ground_map sub_to_ground expr"
+
+definition from_ground :: "'expr\<^sub>G \<Rightarrow> 'expr" where 
+  "from_ground expr\<^sub>G \<equiv> from_ground_map sub_from_ground expr\<^sub>G"
+
+sublocale grounding 
+  where vars = vars and subst = subst and to_ground = to_ground and from_ground = from_ground
+proof unfold_locales
+  have "\<And>expr. is_ground expr \<Longrightarrow> expr \<in> range from_ground"
+  proof-
+    fix expr
+
+    assume "is_ground expr"
+
+    then have "\<forall>sub\<in>to_set expr. sub \<in> range sub_from_ground"
+      by (simp add: sub.is_ground_iff_range_from_ground vars_def)
+
+    then have "\<forall>sub\<in>to_set expr. \<exists>sub\<^sub>G. sub_from_ground sub\<^sub>G = sub"
+      by fast
+
+    then have "\<exists>expr\<^sub>G. from_ground expr\<^sub>G = expr"
+      using map_ground_comp[symmetric] map_id_cong
+      unfolding from_ground_def comp_def
+      by metis
+
+    then show "expr \<in> range from_ground"
+      unfolding from_ground_def
+      by blast
+  qed
+
+  moreover have "\<And>expr var. var \<notin> vars (from_ground expr)"
+  proof
+    fix expr var
+
+    assume "var \<in> vars (from_ground expr)"
+
+    then show False
+      unfolding vars_def from_ground_def
+      using sub.ground_is_ground to_set_from_ground_map by auto
+  qed
+
+  ultimately show "{expr. is_ground expr} = range from_ground"
+    by blast   
+next
+  show "\<And>expr\<^sub>G. to_ground (from_ground expr\<^sub>G) = expr\<^sub>G"
+    using ground_map_id
+    unfolding from_ground_def to_ground_def 
+    by (metis ground_map_comp sub.to_ground_from_ground_id)
+qed
+
+lemma to_set_from_ground: "to_set (from_ground expr) = sub_from_ground ` (to_set_ground expr)"
+  unfolding from_ground_def
+  by (simp add: to_set_from_ground_map)
+
+lemma sub_in_ground_is_ground: 
+  assumes "sub \<in> to_set (from_ground expr)" 
+  shows "sub.is_ground sub"
+  using assms
+  by (simp add: to_set_is_ground)
+
+lemma ground_sub_in_ground: 
+  "sub \<in> to_set_ground expr \<longleftrightarrow> sub_from_ground sub \<in> to_set (from_ground expr)"
+  by (simp add: inj_image_mem_iff sub.inj_from_ground to_set_from_ground)
+
+lemma ground_sub: 
+  "(\<forall>sub \<in> to_set (from_ground expr\<^sub>G). P sub) \<longleftrightarrow> 
+   (\<forall>sub\<^sub>G \<in> to_set_ground expr\<^sub>G. P (sub_from_ground sub\<^sub>G))"
+  by (simp add: to_set_from_ground)
+
+end
+
+locale all_subst_ident_iff_ground_lifting = 
+  finite_variables_lifting 
+  where map = map and id_subst = id_subst +  
+  sub: all_subst_ident_iff_ground 
+  where subst = sub_subst and is_ground = sub.is_ground
+  for map :: "('sub \<Rightarrow> 'sub) \<Rightarrow> 'expr \<Rightarrow> 'expr" and id_subst :: "'var \<Rightarrow> 'base"
+begin
+
+sublocale all_subst_ident_iff_ground where subst = subst and is_ground = is_ground
+proof unfold_locales
+  fix expr 
+
+  show "is_ground expr \<longleftrightarrow> (\<forall>\<sigma>. expr \<cdot> \<sigma> = expr)"
+  proof(rule iffI allI)
+    assume "is_ground expr"
+    then show "\<forall>\<sigma>. expr \<cdot> \<sigma> = expr"
+      by simp
+  next
+    assume all_subst_ident: "\<forall>\<sigma>. expr \<cdot> \<sigma> = expr"
+    
+    show "is_ground expr"
+    proof(rule ccontr)
+      assume "\<not>is_ground expr"
+
+      then obtain sub where sub: "sub \<in> to_set expr" "\<not>sub.is_ground sub"
+        unfolding vars_def
+        by blast
+
+      then obtain \<sigma> where "sub \<cdot>\<^sub>s \<sigma> \<noteq> sub" and "sub \<cdot>\<^sub>s \<sigma> \<notin> to_set expr"
+        using sub.exists_non_ident_subst finite_to_set
+        by blast
+        
+      then show False
+        using sub subst_in_to_set_subst all_subst_ident
+        by metis
+    qed
+  qed
+next
+  fix expr :: 'expr and S :: "'expr set"
+
+  assume finite: "finite S" and not_ground: "\<not>is_ground expr"
+
+  then have finite_subs: "finite (\<Union>(to_set ` insert expr S))"
+    using finite_to_set by blast
+
+  obtain sub where sub: "sub \<in> to_set expr" and sub_not_ground: "\<not>sub.is_ground sub"
+    using not_ground
+    unfolding vars_def
+    by blast
+
+  obtain \<sigma> where \<sigma>_not_ident: "sub \<cdot>\<^sub>s \<sigma> \<noteq> sub" "sub \<cdot>\<^sub>s \<sigma> \<notin> \<Union> (to_set ` insert expr S)"
+    using sub.exists_non_ident_subst[OF finite_subs sub_not_ground]
+    by blast
+
+  then have "expr \<cdot> \<sigma> \<noteq> expr"
+    using sub
+    unfolding subst_def
+    by (simp add: to_set_map_not_ident)
+
+  moreover have "expr \<cdot> \<sigma> \<notin> S"
+    using \<sigma>_not_ident(2) sub to_set_map
+    unfolding subst_def
+    by auto
+
+  ultimately show "\<exists>\<sigma>. expr \<cdot> \<sigma> \<noteq> expr \<and> expr \<cdot> \<sigma> \<notin> S"
+    by blast
+qed
+
+end
+
+end
